coq/minor.v
@@ -1,3 +1,5 @@
+Require Import RelationClasses.
+
 From mathcomp Require Import all_ssreflect.
 Require Import edone finite_quotient preliminaries sgraph.
 
